We want to prove that $\mathrm{P}(k+1)$ is true whenever $\mathrm{P}(k)$ is true, i.e.,

$$
\mathrm{P}(k+1): \mathrm{A}^{k+1}=\left[\begin{array}{cc}
\cos (k+1) \theta & \sin (k+1) \theta \\
-\sin (k+1) \theta & \cos (k+1) \theta
\end{array}\right]
$$

Now

$$
\mathrm{A}^{k+1}=\mathrm{A}^{k} \cdot \mathrm{~A}
$$

Since $\mathrm{P}(k)$ is true, we have

$$
\mathrm{A}^{k+1}=\left[\begin{array}{cc}
\cos k \theta & \sin k \theta \\
-\sin k \theta & \cos k \theta
\end{array}\right]\left[\begin{array}{cc}
\cos \theta & \sin \theta \\
-\sin \theta & \cos \theta
\end{array}\right]
$$

$$
=\left[\begin{array}{cc}
\cos k \theta \cos \theta-\sin k \theta \sin \theta & \cos k \theta \sin \theta+\sin k \theta \cos \theta \\
-\sin k \theta \cos \theta-\cos k \theta \sin \theta & -\sin k \theta \sin \theta+\cos k \theta \cos \theta
\end{array}\right]
$$ (by matrix multiplication)

$$
=\left[\begin{array}{cc}
\cos (k+1) \theta & \sin (k+1) \theta \\
-\sin (k+1) \theta & \cos (k+1) \theta
\end{array}\right]
$$

Thus, $\mathrm{P}(k+1)$ is true whenever $\mathrm{P}(k)$ is true.
Hence, $\mathrm{P}(n)$ is true for all $n \geq 1$ (by the principle of mathematical induction).

## (iii) Proof by cases or by exhaustion

This method of proving a statement $p \Rightarrow q$ is possible only when $p$ can be split into several cases, $r, s, t$ (say) so that $p=r \vee s \vee t$ (where " $\vee$ " is the symbol for "OR").
If the conditionals $\quad r \Rightarrow q$;

$$
s \Rightarrow q
$$

and

$$
t \Rightarrow q
$$

are proved, then $(r \vee s \vee t) \Rightarrow q$, is proved and so $p \Rightarrow q$ is proved.
The method consists of examining every possible case of the hypothesis. It is practically convenient only when the number of possible cases are few.

Example 4 Show that in any triangle ABC ,

$$
a=b \cos \mathrm{C}+c \cos \mathrm{~B}
$$

Solution Let $p$ be the statement "ABC is any triangle" and $q$ be the statement

$$
" a=b \cos \mathrm{C}+c \cos \mathrm{~B} "
$$

Let ABC be a triangle. From A draw AD a perpendicular to BC ( BC produced if necessary).

As we know that any triangle has to be either acute or obtuse or right angled, we can split $p$ into three statements $r, s$ and $t$, where

